src/Relations/ZXbiperm.v
@@ -8,96 +8,197 @@ Import QuantumLib.VectorStates Modulus Kronecker.
 Require Import NFBiperm.
 
 
-(* Section ZX_biperm_foundations_extras *)
+(* NB ncap' and ncup' have inverse interpretations to the diagrams *)
+Definition cap_NF_biperm : NF_biperm := {|
+  lperm' := idn; rperm' := idn;
+  ncup' := 1; 
+  ncap' := 0;
+  nid' := 0;
+|}.
 
-(* Not making these instances for performance and because these 
-   definitions arefully internal and should not be used externally *)
-Lemma change_NF_from_shrink_biperm_eq_of_perm_eq {n m} {f g} 
-  (Hfg : perm_eq (m + n) f g) b : 
-  change_NF_from_shrink_biperm n m f b = 
-  change_NF_from_shrink_biperm n m g b.
+Definition cup_NF_biperm : NF_biperm := {|
+  lperm' := idn; rperm' := idn;
+  ncup' := 0; 
+  ncap' := 1;
+  nid' := 0;
+|}.
+
+Definition wire_NF_biperm : NF_biperm := {|
+  lperm' := idn; rperm' := idn;
+  ncup' := 0; 
+  ncap' := 0;
+  nid' := 1;
+|}.
+
+Definition swap_NF_biperm : NF_biperm := {|
+  lperm' := swap_2_perm; rperm' := idn;
+  ncup' := 0; ncap' := 0;
+  nid' := 2;
+|}.
+
+Lemma cap_NF_biperm_WF : WF_NF_biperm cap_NF_biperm.
 Proof.
-  unfold change_NF_from_shrink_biperm.
-  repeat (apply f_equal_if_precedent_same; 
-    rewrite ?Nat.eqb_eq, ?Nat.eqb_neq; intros; 
-    rewrite ?Hfg by lia;
-    try reflexivity).
+  split; cbn; auto with perm_db.
 Qed.
 
-Lemma grow_NF_of_shrunken_biperm_eq_of_perm_eq {n m} {f g} 
-  (Hfg : perm_eq (m + n) f g) b : 
-  grow_NF_of_shrunken_biperm n m f b = 
-  grow_NF_of_shrunken_biperm n m g b.
+Lemma cup_NF_biperm_WF : WF_NF_biperm cup_NF_biperm.
 Proof.
-  unfold grow_NF_of_shrunken_biperm.
-  repeat (apply f_equal_if_precedent_same; 
-    rewrite ?Nat.eqb_eq, ?Nat.eqb_neq; intros; 
-    rewrite ?Hfg by lia;
-    try reflexivity).
+  split; cbn; auto with perm_db.
 Qed.
 
-(* TODO: Redefine change_fun_to_shrink_biperm 
-  defensively to remove the bipermutation condition. 
-  Should be sufficient to just test f 0 =? 0. *)
-Lemma change_fun_to_shrink_biperm_perm_eq_of_perm_eq_perm_eq {n m}
-  {f f'} (Hf : perm_eq (m + n) f f') {g g'} (Hg : perm_eq (m + n) g g') 
-  (Hfbiperm : bipermutation (m + n) f) :
-  perm_eq (m + n) (change_fun_to_shrink_biperm n m f g)
-    (change_fun_to_shrink_biperm n m f' g').
+Lemma wire_NF_biperm_WF : WF_NF_biperm wire_NF_biperm.
 Proof.
-  unfold change_fun_to_shrink_biperm.
-  bdestruct (m =? 0).
-  - bdestructΩ'.
-    pose proof (Hfbiperm 0 ltac:(lia)).
-    rewrite <- Hf by lia.
-    rewrite 2!compose_assoc.
-    now rewrite Hg.
-  - rewrite <- Hf by lia.
-    bdestructΩ';
-    rewrite 2!compose_assoc;
-    pose proof (Hfbiperm 0 ltac:(lia)).
-    + rewrite <- (stack_perms_WF_idn m n (swap_perm 1 _ _))
-        by cleanup_perm_inv.
-      now rewrite Hg.
-    + now rewrite Hg.
+  split; cbn; auto with perm_db.
 Qed.
 
-Lemma NF_of_biperm_rec_eq_of_perm_eq fuel : forall n m f g, 
-  perm_eq (m + n) f g -> bipermutation (m + n) f ->
-  NF_of_biperm_rec fuel n m f = NF_of_biperm_rec fuel n m g.
+Lemma swap_NF_biperm_WF : WF_NF_biperm swap_NF_biperm.
 Proof.
-  induction fuel; [easy|].
-  intros n m f g Hfg Hf.
+  split; cbn; auto with perm_db.
+Qed.
+
+Lemma matrix_of_empty_NF_biperm : 
+  matrix_of_NF_biperm empty_NF_biperm = ⟦ ⦰ ⟧.
+Proof.
+  apply matrix_of_biperm_0_0.
+Qed.
+
+Lemma matrix_of_cap_NF_biperm : 
+  matrix_of_NF_biperm cap_NF_biperm = ⟦ Cap ⟧.
+Proof.
+  prep_matrix_equivalence.
+  by_cell; reflexivity.
+Qed.
+
+Lemma matrix_of_cup_NF_biperm : 
+  matrix_of_NF_biperm cup_NF_biperm = ⟦ Cup ⟧.
+Proof.
+  prep_matrix_equivalence.
+  by_cell; reflexivity.
+Qed.
+
+Lemma matrix_of_wire_NF_biperm : 
+  matrix_of_NF_biperm wire_NF_biperm = ⟦ — ⟧.
+Proof.
+  prep_matrix_equivalence.
+  by_cell; reflexivity.
+Qed.
+
+Lemma matrix_of_swap_NF_biperm : 
+  matrix_of_NF_biperm swap_NF_biperm = ⟦ ⨉ ⟧.
+Proof.
+  prep_matrix_equivalence.
+  by_cell; reflexivity.
+Qed.
+
+Inductive ZXbiperm : forall {n m}, ZX n m -> Prop :=
+  | BipermEmpty : ZXbiperm Empty
+  | BipermWire : ZXbiperm Wire 
+  | BipermCup : ZXbiperm Cup
+  | BipermCap : ZXbiperm Cap
+  | BipermSwap : ZXbiperm Swap
+  | BipermCompose {n m o} {zx0 : ZX n m} {zx1 : ZX m o} : 
+    ZXbiperm zx0 -> ZXbiperm zx1 -> ZXbiperm (zx0 ⟷ zx1)
+  | BipermStack {n m o p} {zx0 : ZX n m} {zx1 : ZX o p} : 
+    ZXbiperm zx0 -> ZXbiperm zx1 -> ZXbiperm (zx0 ↕ zx1).
+
+Fixpoint NF_of_zx {n m} (zx : ZX n m) : NF_biperm :=
+  match zx with 
+  | ⦰ => empty_NF_biperm
+  | Cup => cup_NF_biperm
+  | Cap => cap_NF_biperm
+  | — => wire_NF_biperm
+  | ⨉ => swap_NF_biperm
+  | zx0 ↕ zx1 => stack_NF_biperms (NF_of_zx zx0) (NF_of_zx zx1)
+  | zx0 ⟷ zx1 => compose_NF_biperms (NF_of_zx zx0) (NF_of_zx zx1)
+  (* Junk cases: *)
+  | Box => empty_NF_biperm
+  | X_Spider _ _ _ => empty_NF_biperm
+  | Z_Spider _ _ _ => empty_NF_biperm
+  end.
+
+Lemma NF_insize_compose_NF_biperms b c  
+  (Hb : WF_NF_biperm b) (Hc : WF_NF_biperm c) 
+  (Hbc : NF_outsize b = NF_insize c) : 
+  NF_insize (compose_NF_biperms b c) = NF_insize b.
+Proof.
+  unfold compose_NF_biperms.
   cbn.
-  bdestruct (m =? 0).
-  - apply f_equal_if_precedent_same; [easy|].
-    rewrite Nat.eqb_neq; intros Hn.
-    rewrite (change_NF_from_shrink_biperm_eq_of_perm_eq Hfg).
-    f_equal.
-    rewrite (grow_NF_of_shrunken_biperm_eq_of_perm_eq Hfg).
-    f_equal.
-    apply IHfuel.
-    + rewrite Nat.add_0_l.
-      replace (n - 2) with (n - 1 - 1) by lia.
-      bdestruct (n =? 1); [subst; intros k Hk; lia|].
-      apply contract_perm_perm_eq_of_perm_eq; [lia|].
-      apply contract_perm_perm_eq_of_perm_eq; [lia|].
-      subst. 
-      now apply (change_fun_to_shrink_biperm_perm_eq_of_perm_eq_perm_eq Hfg).
-    (* + pose proof  *)
-    Admitted.
+  rewrite double_add, <- Nat.add_assoc.
+  rewrite ncup_ncup_nid_compose_n_caps_NF_l;
+  [cbn; lia..|].
+  apply compose_perm_l_NF_biperm_WF;
+  [apply Hc | rewrite <- Hbc; apply Hb].
+Qed.
 
-    
-    
-
-
-(* Add Parametric Morphism n m : (NF_of_biperm n m)
-  with signature perm_eq (m + n) ==> eq as NF_of_biperm_eq_of_perm_eq.
+Lemma NF_outsize_compose_NF_biperms b c  
+  (Hb : WF_NF_biperm b) (Hc : WF_NF_biperm c) 
+  (Hbc : NF_outsize b = NF_insize c) : 
+  NF_outsize (compose_NF_biperms b c) = NF_outsize c.
 Proof.
-  intros f g H *)
+  unfold compose_NF_biperms.
+  cbn.
+  rewrite ncap_ncap_nid_compose_n_caps_NF_l;
+  [cbn; lia..|].
+  apply compose_perm_l_NF_biperm_WF;
+  [apply Hc | rewrite <- Hbc; apply Hb].
+Qed.
 
+Lemma NF_of_zx_size_and_WF {n m} (zx : ZX n m) (H : ZXbiperm zx) : 
+  WF_NF_biperm (NF_of_zx zx) /\ 
+  NF_insize (NF_of_zx zx) = n /\ 
+  NF_outsize (NF_of_zx zx) = m.
+Proof.
+  induction H; cbn [NF_of_zx].
+  - split; [|easy]; apply empty_NF_biperm_WF.
+  - split; [|easy]; apply wire_NF_biperm_WF.
+  - split; [|easy]; apply cup_NF_biperm_WF.
+  - split; [|easy]; apply cap_NF_biperm_WF.
+  - split; [|easy]; apply swap_NF_biperm_WF.
+  - split. 
+    + apply compose_NF_biperms_WF; lia + easy.
+    + rewrite NF_insize_compose_NF_biperms by lia + easy.
+      rewrite NF_outsize_compose_NF_biperms by lia + easy.
+      lia.
+  - split; [|cbn; lia..].
+    apply stack_NF_biperms_WF; easy.
+Qed.
 
+Lemma NF_of_zx_WF {n m} (zx : ZX n m) (H : ZXbiperm zx) : 
+  WF_NF_biperm (NF_of_zx zx).
+Proof. now apply NF_of_zx_size_and_WF. Qed.
 
+Lemma NF_insize_NF_of_zx {n m} (zx : ZX n m) (H : ZXbiperm zx) : 
+  NF_insize (NF_of_zx zx) = n.
+Proof. now apply NF_of_zx_size_and_WF. Qed.
+
+Lemma NF_outsize_NF_of_zx {n m} (zx : ZX n m) (H : ZXbiperm zx) : 
+  NF_outsize (NF_of_zx zx) = m.
+Proof. now apply NF_of_zx_size_and_WF. Qed.
+
+Lemma NF_of_zx_correct {n m} (zx : ZX n m) (H : ZXbiperm zx) : 
+  ⟦ zx ⟧ [∝] matrix_of_NF_biperm (NF_of_zx zx).
+Proof.
+  induction H; cbn [NF_of_zx].
+  - now rewrite matrix_of_empty_NF_biperm.
+  - now rewrite matrix_of_wire_NF_biperm.
+  - now rewrite matrix_of_cup_NF_biperm.
+  - now rewrite matrix_of_cap_NF_biperm.
+  - now rewrite matrix_of_swap_NF_biperm.
+  - destruct (NF_of_zx_size_and_WF zx0 ltac:(assumption))
+      as (HWF1 & Hin1 & Hout1).
+    destruct (NF_of_zx_size_and_WF zx1 ltac:(assumption))
+      as (HWF2 & Hin2 & Hout2).
+    rewrite compose_NF_biperms_correct by assumption + lia.
+    rewrite Hin1, Hin2, Hout2.
+    now apply Mmult_mat_prop_proper.
+  - destruct (NF_of_zx_size_and_WF zx0 ltac:(assumption))
+      as (HWF1 & Hin1 & Hout1).
+    destruct (NF_of_zx_size_and_WF zx1 ltac:(assumption))
+      as (HWF2 & Hin2 & Hout2).
+    rewrite stack_NF_biperms_correct by assumption + lia.
+    rewrite Hin1, Hin2, Hout1, Hout2.
+    now apply kron_mat_prop_proper.
+Qed.
 
 
 
